ironfleet/src/Dafny/Distributed/Protocol/RSL/CommonProof/ReplyCache.i.dfy
@@ -31,9 +31,7 @@ predicate ReplyCacheObjectInv(cache:ReplyCache, client:NodeIdentity)
 
 predicate ReplyCacheStateInv(ps:RslState, client:NodeIdentity)
 {
-  && (forall p :: p in ps.environment.sentPackets && p.src in ps.constants.config.replica_ids && p.msg.RslMessage_AppStateSupply? ==>
-           ReplyCacheObjectInv(p.msg.reply_cache, client))
-  && (forall idx :: 0 <= idx < |ps.replicas| ==> ReplyCacheObjectInv(ps.replicas[idx].replica.executor.reply_cache, client))
+  forall idx :: 0 <= idx < |ps.replicas| ==> ReplyCacheObjectInv(ps.replicas[idx].replica.executor.reply_cache, client)
 }
 
 lemma lemma_ReplyCacheStateInv(
@@ -74,34 +72,7 @@ lemma lemma_ReplyCacheStateInv(
       else
       {
         var ios :| RslNextOneReplica(ps, ps', idx, ios);
-        if exists inp:LPacket<NodeIdentity, RslMessage> ::
-             && LIoOpReceive(inp) in ios
-             && inp.msg.RslMessage_AppStateSupply?
-             && inp.src in s.executor.constants.all.config.replica_ids
-             && LReplicaNextProcessAppStateSupply(s, s', inp, [])
-        {
-          var inp:LPacket<NodeIdentity, RslMessage> :|
-              && LIoOpReceive(inp) in ios
-              && inp.msg.RslMessage_AppStateSupply?
-              && inp.src in s.executor.constants.all.config.replica_ids
-              && LReplicaNextProcessAppStateSupply(s, s', inp, []);
-          lemma_PacketProcessedImpliesPacketSent(ps, ps', idx, ios, inp);
-          assert ReplyCacheObjectInv(inp.msg.reply_cache, client);
-          assert ReplyCacheObjectInv(cache', client);
-        }
-        else
-        {
-          assert ReplyCacheObjectInv(cache', client);
-        }
-      }
-    }
-
-    forall p | p in ps'.environment.sentPackets && p.src in ps.constants.config.replica_ids && p.msg.RslMessage_AppStateSupply?
-      ensures ReplyCacheObjectInv(p.msg.reply_cache, client)
-    {
-      if p !in ps.environment.sentPackets
-      {
-        var idx, ios := lemma_ActionThatSendsAppStateSupplyIsProcessAppStateRequest(ps, ps', p);
+        assert ReplyCacheObjectInv(cache', client);
       }
     }
   }
